src/lang/syntax.v
@@ -1,3 +1,5 @@
+(* The definition of the _syntax_ of NvmLang. *)
+
 From stdpp Require Export binders strings.
 From stdpp Require Import countable.
 From iris.algebra Require Import ofe.
@@ -321,6 +323,9 @@ Module syntax.
   Qed.
   Global Instance val_countable : Countable val.
   Proof. refine (inj_countable of_val to_val _); auto using to_of_val. Qed.
+
+  Global Instance val_inhabited : Inhabited val := populate (LitV LitUnit).
+  Global Instance expr_inhabited : Inhabited expr := populate (Val inhabitant).
 
   Canonical Structure valO := leibnizO val.
   Canonical Structure exprO := leibnizO expr.
